\documentclass[class=ctexart,crop=false]{standalone}

\input{../mathpre}
\begin{document}

\begin{enumerate}[label=(\Roman*)]
    \item 证明：\\
    设直线$AB:x=ky+\frac{1}{2},l_1:y=y_1,l_2:y=y_2$\\
    则:$A:(\frac{y_1^2}{2},y_1),B:(\frac{y_2^2}{2},y_2),
    R:(-\frac{1}{2},\frac{y_1+y_2}{2}),F:(\frac{1}{2},0),
    P:(-\frac{1}{2},y_1),Q:(-\frac{1}{2},y_2)$\\
    则:$k_{RA}=\frac{y_1-\frac{y_1+y_2}{2}}{\frac{y_1^2}{2}+\frac{1}{2}}
    =\frac{y_1-y_2}{y_1^2+1},
    k_{QF}=\frac{0-y_2}{\frac{1}{2}+\frac{1}{2}}=-y_2$\\
    且 $y_1,y_2$满足:
    \begin{empheq}[left=\empheqlbrace]{align}
        C:y^2&=2x\\
        AB:x&=ky+\frac{1}{2}
    \end{empheq}
    故有: $y^2-2ky-1=0$\\
    则: $y_1y_2=-1 \Rightarrow y_2=-\frac{1}{y_2}$ \\
    故:$k_{RA}=\frac{y_1+\frac{1}{y_2}}{y_1^2+1}=\frac{y_1^2+1}{y_1(y_1^2+y_1)}
    =\frac{1}{y_1}=-y_2=k_{QF}$\\
    证毕
    \item 解：\\
    易知 $S_{\triangle PQF}=\frac{1}{2}(y_1-y_2)[\frac{1}{2}-(-\frac{1}{2})]=\frac{y_1-y_2}{2}$\\
    记 $AB$与 $x$轴交于 $D$点,设 $AB:x=ky+b$,则$D:(b,0)$\\
    故 $S_{\triangle ABF}=\frac{1}{2}|b-\frac{1}{2}|(y_1-y_2)$\\
    由 $S_{\triangle PQF}=2S_{\triangle ABF}\Rightarrow \frac{y_1-y_2}{2}=|b-\frac{1}{2}|(y_1-y_2)$
    则:$|b-\frac{1}{2}|=\frac{1}{2}$\\
    故 $b=1$或 $b=0$(舍去)\\
    且 $y_1,y_2$满足:
    \begin{empheq}[left=\empheqlbrace]{align}
        C:y^2&=2x\\
        AB:x&=ky+1
    \end{empheq}
    故有 $y^2-2ky-2=0$\\
    则:$y_1y_2=-2,y_1+y_2=2k$\\
    则:$\frac{y_1^2}{2}+\frac{y_2^2}{2}=\frac{1}{2}[(y_1+y_2)^2-2y_1y_2]=2k^2+2$\\
    故$AB$中点的轨迹方程为 $x=k^2+1=y^2+1$,即 $y^2=x-1$
\end{enumerate}

\end{document}