\documentclass[class=ctexart,crop=false]{standalone}

\input{../mathpre}
\begin{document}
解:
\begin{enumerate}[label=(\Roman*)]
    \item $f'(x)=-2\alpha \sin 2x+(\alpha-1)(-\sin x)=-4\alpha\sin x\cos x-\alpha\sin x+\sin x$;
    \item 
    ($|f(x)|=|\alpha \cos 2x+(\alpha-1)(\cos x +1)|\leqslant a+2(a-1)=3a-2 $)\\
       $\begin{aligned}[t]
       f(x)&=2\alpha cos^2(x)-\alpha+\alpha cos x+\alpha -cos x -1\\
       &=2\alpha(\cos x +\frac{\alpha-1}{4\alpha})^2-\frac{\alpha^2-2\alpha+1}{8a}-1\\
       &=2\alpha(\cos x +\frac{\alpha-1}{4\alpha})^2-\frac{\alpha^2+6\alpha+1}{8a}\\
       \end{aligned}$\\
       记 $t=\cos x,$则$t \in [-1,1],f(x)=g(t)=2\alpha(t-\frac{1-\alpha}{4\alpha})^2-\frac{\alpha^2+6\alpha+1}{8a}$\\
       可知 $g(t)$为关于$t$ 的二次函数,开口向上,极小值 $A_1=-\frac{\alpha^2+6\alpha+1}{8a}$\\
       由 $t=\cos x\in [-1,1]$,若 $\frac{1-\alpha}{4\alpha}\in [-1,1],$
       即 $\alpha \geqslant \frac{1}{5}$时:极值在区间内\\
       $\cos x=1$时:$g(1)=3\alpha -2,\cos x=-1$时:$g(-1)=\alpha$\\
       则:
    \begin{enumerate}[label=(\roman*)]
        \item $0<\alpha\leqslant \frac{1}{5}$时,:\\
            $|g(t)|$的最大值在端点取得\\
            又$|g(-1)|-|g(1)|=\alpha -2+3\alpha=4\alpha-2<0$\\
            故此时 $A=|g(1)|=|3\alpha-2|=2-3\alpha$
        \item $\alpha>\frac{1}{5} $时:\\
            $A$为$|A_1|,|g(1)|,|g(-1)|$中的最大值\\
            由 $a>0$,故$\begin{aligned}[t]
                |A_1|-|g(-1)|&=\frac{\alpha^2+6\alpha+1}{8\alpha}-\alpha\\
                            &=\frac{-7\alpha^2+6\alpha+1}{8\alpha}\\
                            &=\frac{(7\alpha+1)(1-\alpha)}{8\alpha}
                \end{aligned}$\\ 
            \begin{enumerate}[label=(\arabic*)]
                \item $a\geqslant 1$时:\\
                $|g(-1)|\geqslant|A_1|\\
                |g(1)|-|g(-1)|=3\alpha-2-\alpha=2\alpha-2\geqslant0$\\
                故此时 $A=3\alpha-2$                
                \item $a < 1$时:\\
                    $|g(-1)|<|A_1|\\
                    \begin{aligned}[t]
                        |A_1|-|g(1)|&=\frac{\alpha^2+6\alpha+1}{8a}-2+3\alpha\\
                            &=\frac{25\alpha^2-10\alpha+1}{8\alpha}\\
                            &=\frac{(5\alpha-1)^2}{8\alpha}\geqslant 0\\
                    \end{aligned}\\$
                故此时 $A=|A_1|=\frac{\alpha^2+6\alpha+1}{8\alpha}$\\
                综上,$A=
                    \begin{cases}
                        2-3\alpha &, \alpha \leqslant \frac{1}{5}\\
                        \frac{\alpha^2+6\alpha+1}{8\alpha} &,\frac{1}{5}<\alpha<1\\
                        3\alpha-2 &,\alpha \geqslant 1\\
                    \end{cases}$
            \end{enumerate}
        \end{enumerate}
    \item  证明:\\
        $|f'(x)|=|-2\alpha \sin 2x -(\alpha -1)\sin x|<2\alpha+|\alpha-1|$
        \begin{enumerate}
            \item $\alpha \geqslant 1$时:\\
                $|f'(x)|-2A<3\alpha-1-6\alpha+4=3-3\alpha\leqslant 0$
            \item $\frac{1}{5}< \alpha<1$时:\\
            $\begin{aligned}[t]
                |f'(x)|-2A&<\alpha+1-\frac{\alpha^2+6\alpha+1}{4\alpha}\\
                &=\frac{3\alpha^2-2\alpha-1}{4\alpha}\\
                &=\frac{(3\alpha+1)(\alpha-1)}{4\alpha}<0\\
            \end{aligned}$\\
            \item $0<\alpha\leqslant \frac{1}{5}$时:\\
            $|f'(x)|-2A<\alpha+1-4+6\alpha=7\alpha-3<0$
        \end{enumerate}
        综上，$|f'(x)|\leqslant 2A$
\end{enumerate}

\end{document}