\documentclass[class=ctexart,crop=false]{standalone}

\input{../../mathpre}
\begin{document}
解:显然 $x>0$
\begin{enumerate}[label=(\arabic*)]
    \item 
    由题意 $a\leqslant \frac{e^x}{x}-\ln{x}+x$\\
    记 $g(x)=\frac{e^x}{x}-\ln{x}+x$\\
    则 $\begin{aligned}[t]
        g'(x)&=\frac{xe^x-e^x}{x^2}-\frac{1}{x}+1\\
        &=\frac{e^x(x-1)+x(x-1)}{x^2}\\
        &=\frac{(e^x+x)(x-1)}{x}\\
    \end{aligned}$ 
    $x<1$时 $g(x)<0$,$x>1$时 $g(x)>0$
    故 $g(x)$ 在 $x=1$ 处取得最小值 $g(1)=1+e$.\\
    故 $a \leqslant 1+e$
    \item   不妨设 $0<x_1<1<x_2$\\
            $x_1x_2<1\iff x_1<\frac{1}{x_2}<1$\\
            由1知:$x<1$时$,f(x)$单调递减\\
            则$x_1<\frac{1}{x_2}\Leftrightarrow f(\frac{1}{x_2})<f(x_1)=0=f(x_2)$\\
            记 $\phi(x)=f(x)-f(\frac{1}{x}),x\in (0,1]$\\
            $\begin{aligned}[t]
                \phi '(x)&=\frac{(e^x+x)(x-1)}{x}-\frac{(e^x+x)(x-1)}{x}(\frac{-1}{x^2})\\
                        &=\frac{(e^x+x)(x-1)}{x}(\frac{x^2+1}{x^2})\\
            \end{aligned}$\\
            故 $\phi'(x)<0,\phi(x)$单调递减\\
            $\phi(1)=f(1)-f(1)=0$\\
            故 $x\in (0,1)$时 $\phi(x)>\phi(1)=0\\
            \Rightarrow f(x_1)=f(x_2)>f(\frac{1}{x_2})\\
            \Rightarrow x_1<\frac{1}{x_2}\Rightarrow x_1x_2<1$
\end{enumerate}
\end{document}